Solution.v
@@ -1,0 +1,46 @@
+Require Import Preloaded Coq.Lists.List VST.floyd.proofauto.
+
+Lemma bt_invert_involution : forall (A : Type) (tree : bt A),
+  bt_invert (bt_invert tree) = tree.
+Proof. intros A tree; induction tree; simpl; congruence. Qed.
+
+Lemma bt_invert_inorder : forall (A : Type) (tree : bt A),
+  bt_inorder (bt_invert tree) = rev (bt_inorder tree).
+Proof.
+  intros A tree; induction tree; simpl; auto.
+  rewrite IHtree1, IHtree2, rev_app_distr; simpl.
+  now rewrite <- app_assoc.
+Qed.
+
+Lemma btrep_local_facts: forall sigma p,
+   btrep sigma p |--
+   !! (is_pointer_or_null p /\ (p=nullval <-> sigma=bt_leaf)).
+Proof.
+  induction sigma; intros.
+  - unfold btrep.
+    entailer!.
+    split; auto.
+  - unfold btrep; fold btrep.
+    Intros y z.
+    entailer!.
+    split; intros H3.
+    + subst p.
+      eapply field_compatible_nullval; eauto.
+    + discriminate.
+Qed.
+
+#[export] Hint Resolve btrep_local_facts : saturate_local.
+
+Lemma btrep_valid_pointer: forall sigma p,
+   btrep sigma p |-- valid_pointer p.
+Proof.
+  destruct sigma; intros; unfold btrep; fold btrep.
+  - entailer!.
+  - Intros y z.
+    entailer!.
+Qed.
+
+#[export] Hint Resolve btrep_valid_pointer : valid_pointer.
+
+Lemma body_invert: semax_body Vprog Gprog f_invert invert_spec.
+Proof. Admitted.
